empty

Isabelle/5. Advanced/Ex5_1.thy
@@ -6,11 +6,231 @@ primrec insort :: "nat \<Rightarrow> nat list \<Rightarrow> nat list " where
   "insort val [] = [val]"|
   "insort val (x#xs) = (if val \<le> x then val#x#xs else x # insort val xs)"
   
-  
-fun sorted :: "nat list \<Rightarrow> bool" where 
-  "sorted [] = True"|
-  "sorted [x] = True"|
-  "sorted (x#y#xs) =  ((x \<le>  y) \<and>  sorted (y#xs))"
-  
-  
-  
+primrec le :: "nat \<Rightarrow> nat list \<Rightarrow> bool" where 
+  "le _ [] =  True"|
+  "le val (x#xs) = ((val \<le> x)  \<and>   le val xs)"
+
+primrec sorted :: "nat list \<Rightarrow> bool" where 
+"sorted [] = True"|
+"sorted (x#xs) = (le  x xs \<and> sorted xs)"
+
+primrec sort :: "nat list \<Rightarrow> nat list" where 
+  "sort [] = [] "|
+  "sort (x#xs) = insort x (sort xs)"
+
+
+
+lemma lem1 [simp]: "x \<le> y \<Longrightarrow> le y xs \<longrightarrow> le x xs" 
+proof (induction xs)
+  case Nil
+  then show ?case by simp
+next
+  case (Cons a xs)
+  then show ?case by (cases "y \<le> a"; simp)
+qed
+
+lemma helper:"le x xs \<Longrightarrow> insort x xs = x # xs" by (induction xs ; simp)
+
+lemma helper2: "le a xs \<Longrightarrow> a \<le> x \<Longrightarrow> le a (insort x xs)"
+proof (induction xs)
+  case Nil
+  then show ?case by simp
+next
+  case (Cons aa xs)
+  then show ?case by (cases "a \<le> aa" ; simp)
+qed
+
+lemma helper3:"\<not> le a xs \<Longrightarrow> le  a (insort x xs) = False" by (induction xs; simp)
+
+
+lemma helper4:"sorted (insort x xs) = sorted xs"
+proof (induction xs)
+  case Nil
+  then show ?case by simp
+next
+  case (Cons a xs)
+  assume hyp:"sorted (Ex5_1.insort x xs) = sorted xs"
+  then show ?case 
+  proof (cases "x \<le> a")
+    case True
+    then show ?thesis by (cases "le a xs"; simp)
+  next
+    case False
+    assume c1:"\<not> x \<le> a"
+    hence tmp:"x > a" by simp
+    then show ?thesis 
+    proof (cases "le x xs")
+      case True
+      assume c2:"le x xs"
+      have tmp2:"a \<le> x" using tmp by simp
+      have "sorted (Ex5_1.insort x (a # xs)) = sorted (a # Ex5_1.insort x  xs)" using c1 by simp
+      also have "\<dots> = sorted (a # x # xs)" using helper c2 by simp
+      also have "\<dots> = (le a (x#xs)  \<and> sorted (x # xs))" by simp
+      also have "\<dots> = ((a \<le> x \<and> le a xs) \<and> sorted (x #xs))" by simp
+      also have "\<dots> = (le a xs \<and> sorted (x#xs))" using c1 by simp
+      also have "\<dots> = sorted xs" using c2 tmp2 by simp
+      finally have a:"sorted (Ex5_1.insort x (a # xs)) = sorted xs" by assumption
+
+      have  "Ex5_1.sorted (a # xs) = (le a xs \<and> sorted xs)" by simp
+      also have "\<dots> = sorted xs" using tmp2 c2 by simp
+      
+      finally show ?thesis using a by simp
+    next
+      case False
+      assume c2:"\<not> le x xs"
+      show ?thesis  
+      proof  (cases "le a xs")
+        case True
+        then show ?thesis using c1 hyp helper2 by simp
+      next
+        case False
+        assume c3:"\<not>le a xs"
+        have f1:"sorted (a # xs)  =  (le a xs \<and> sorted xs)" by simp
+        also have "\<dots> = (False \<and> sorted xs)" using c3 by simp
+        also have "\<dots> = False" by simp
+        finally have res1:"sorted (a # xs) = False" by assumption
+
+        have "sorted (insort x (a # xs)) = sorted (a # insort x xs)" using c1 by simp
+        also have "\<dots> =False" using c3 helper3 by simp
+        finally show ?thesis using res1 by simp
+      qed
+    qed
+  qed
+qed
+
+
+
+theorem "sorted (sort xs)" 
+proof (induction xs)
+  case Nil
+  then show ?case by simp
+next
+  case (Cons a xs)
+  assume "sorted (sort xs)"
+  have "sorted (sort (a#xs)) = sorted (insort a (sort xs))" by simp
+  then show ?case using helper4 Cons.IH by simp
+qed
+
+primrec count :: "'a list \<Rightarrow> 'a \<Rightarrow> nat" where 
+  "count [] _ = 0"|
+  "count (x#xs) val = (if val = x then 1 else 0) + count xs val"
+
+lemma helper5: "count (insort x xs) y= count (x# xs) y" by (induction xs ; auto)
+
+theorem "count (sort xs) x = count xs x" by (induction xs ; auto simp add : helper5)
+
+
+datatype bintree = leaf | node nat (l:"bintree") (r:"bintree")
+
+primrec tge :: "nat \<Rightarrow> bintree \<Rightarrow> bool" where 
+"tge _ leaf = True"|
+"tge val (node val2 lft rgt) = (val \<ge> val2 \<and> tge val lft \<and> tge val rgt)"
+
+primrec tle :: "nat \<Rightarrow> bintree \<Rightarrow> bool" where 
+"tle _ leaf = True"|
+"tle val (node val2 lft rgt) = (val \<le> val2 \<and> tle val lft \<and> tle val rgt)"
+
+primrec tsorted :: "bintree \<Rightarrow> bool" where 
+"tsorted leaf = True"|
+"tsorted (node val lft rgt) =  (tsorted lft \<and> tsorted rgt \<and> tge val lft \<and>  tle val rgt)"
+
+primrec ins :: "nat \<Rightarrow> bintree \<Rightarrow> bintree" where 
+"ins val leaf = node val leaf leaf"|
+"ins val (node val2 lft rgt) = (if val < val2 then node val2 (ins val lft ) rgt else node val2 lft (ins val rgt))"
+
+primrec tree_of :: "nat list \<Rightarrow> bintree" where 
+"tree_of [] = leaf"|
+"tree_of (x#xs) = ins x (tree_of xs)"
+
+lemma helper6:"x < y \<Longrightarrow> tge y t \<Longrightarrow> tge y (ins x t)" by (induction t ; simp)
+
+lemma helper7:"x \<ge> y \<Longrightarrow> tle y t \<Longrightarrow> tle y (ins x t)" by (induction t; simp)
+
+lemma helper8:"\<not>tge x t \<Longrightarrow>  \<not>tge x (ins y t)" by (induction t ; auto)
+
+lemma helper9:"\<not>tle x t \<Longrightarrow> \<not>tle x (ins y t)" by (induction t; auto)
+
+lemma helper10: "tsorted (ins x t) = tsorted t" 
+proof (induction t)
+  case leaf
+  then show ?case by simp
+next
+  case (node x1 t1 t2)
+  assume hyp1:"tsorted (ins x t1) = tsorted t1"
+     and hyp2:"tsorted (ins x t2) = tsorted t2"
+  show ?case  
+  proof (cases "x < x1")
+    case True
+    assume c1:"x < x1"
+    have tmp:"tsorted (ins x (node x1 t1 t2)) = tsorted  (node x1 (ins x t1) t2)" by (simp add : True)
+    show ?thesis 
+    proof (cases "tge x1 t1")
+      case True
+      then show ?thesis using hyp1 helper6[of x x1 t1] c1 by (cases "tle x1 t1" ; simp) 
+    next
+      case False
+      then show ?thesis using helper8[of x1 t1 x] c1 by (cases "tle x1 t2" ; simp)
+    qed
+  next
+    case False
+    assume "\<not> x < x1"
+    hence c1:"x1 \<le> x" by simp
+    then show ?thesis using helper7[of x1 x t2] helper9[of x1 t2 x] hyp2 by (cases "tge x1 t1" ; cases "tle x1 t2" ; auto) 
+  qed
+qed
+
+theorem [simp] : "tsorted (tree_of xs)" 
+proof (induction xs)
+  case Nil
+  then show ?case by simp
+next
+  case (Cons a xs)
+  then show ?case using helper10 by simp
+qed
+
+primrec tcount :: "bintree \<Rightarrow> nat  \<Rightarrow> nat" where 
+"tcount leaf _  = 0"|
+"tcount (node val2 lft rgt) val = (if val = val2 then 1 else 0) + tcount lft val + tcount rgt val"
+
+lemma helper11: "tcount (ins x t) y = (if y = x then 1 else 0) + tcount t y" by (induction t ; auto)
+
+theorem "tcount (tree_of xs) x = count xs x" using helper11 by (induction xs ; simp)
+
+primrec list_of :: "bintree \<Rightarrow> nat list" where 
+"list_of leaf = []"|
+"list_of (node val lft rgt) = list_of lft @ val # list_of rgt"
+(*
+lemma helper12:"sorted (xs @ ys) = (sorted xs \<and> sorted ys)" quickcheck
+*)
+lemma helper111:"list_of (tree_of xs) = sort xs" 
+proof (induction xs)
+  case Nil
+  then show ?case by simp
+next
+  case (Cons a xs)
+  then show ?case 
+qed
+
+lemma helper12:"sorted (list_of (ins x t)) = sorted (list_of t)" 
+proof (induction t)
+  case leaf
+  then show ?case by simp
+next
+  case (node x1 t1 t2)
+  assume hyp1:"sorted (list_of (ins x t1)) = sorted (list_of t1)"
+     and hyp2:"sorted (list_of (ins x t2)) = sorted (list_of t2)"
+(*  have "sorted (list_of (ins x (node x1 t1 t2))) =  sorted (list_of t1 @ x1 # list_of())"*)
+  show ?case 
+  proof (cases "x < x1")
+    case True
+    hence  "sorted (list_of (ins x (node x1 t1 t2))) =  sorted (list_of (ins x t1) @ x1 # list_of t2)" by simp
+    then show ?thesis 
+  next
+    case False
+    then show ?thesis sorry
+  qed
+
+qed
+
+
+theorem "sorted (list_of (tree_of xs))" 
